Re-work the test slightly so that it extracts via KreMLin

examples/low-level/crypto/Plain.fst
@@ -66,6 +66,10 @@ abstract type plainBuffer (i:id) (l:plainLen) = b:lbuffer l
 val as_buffer: #i:id -> #l:plainLen -> pb: plainBuffer i l -> GTot(lbuffer l)
 let as_buffer #i #l pb = pb
 
+// for tests
+val unsafe_hide_buffer: i:id -> #l:plainLen -> b:lbuffer l -> Tot (plainBuffer i l)
+let unsafe_hide_buffer i #l b = b
+
 // usage?
 val hide_buffer: i:id -> #l:plainLen -> b:lbuffer l -> GTot (plainBuffer i l)
 let hide_buffer i #l b = b
